Axioms in certicoq:
So far I have added a new Term constructor (TAx : Term -> Term).  The
argument to TAx is the axiom's type, so this is like having a single
undefined value shared by all axioms.  The various evaluators simply
block on this constant.

I've carried this approach through all of L1, L2 and L3.  This should
evaluate the same as Coq.  On Abishek's example

    Axiom feq1 : (fun x:nat => x) = (fun x:nat => x+x-x).

(with fuel-driven weak cbv evaluation) in L1, L2, and L3, the current
version does indeed agree with Coq.

NOTE: My tests (test_wcbvEval.v in directories L1, L2 and L3) compare

- quoting and translation to Ln followed by evaluation in Ln, 
- evaluation (in Coq) followed by quoting and and translation to Ln.

Once a test rig is set up for each language (a few lines of Coq),
examples are tested with [vm_compute; reflexivity].

If we allow axioms to not block evaluation (e.g. if every match with
only one branch always steps), then this easy testing no longer works.

"make"ing the whole project now fails on

File "./L4_deBruijn/L3_to_L4.v", line 46, characters 2-1365:
Error: Non exhaustive pattern-matching: ...

Since L4 doesn't yet have a TAx term constructor.

theories/L1_MalechaQuoted/program.v
@@ -1,5 +1,4 @@
 
-
 Require Import Lists.List.
 Require Import Strings.String.
 Require Import Strings.Ascii.
@@ -30,16 +29,16 @@ Inductive envClass :=
 | ecTrm (_:Term)
 | ecTyp (_:itypPack).
 
-(** An environ is a list of definitions.
-***  Currently ignoring Axioms
-**)
+(** An environ is a list of axioms and
+*** definitions of terms and inductive types
+***)
 Definition environ := list (string * envClass).
 Record Program : Type := mkPgm { main:Term; env:environ }.
 
 Inductive WFaEc: envClass -> Prop :=
 | wfaecTrm: forall t, WFapp t -> WFaEc (ecTrm t)
 | wfaecTyp: forall i, WFaEc (ecTyp i).
-
+    
 Inductive WFaEnv: environ -> Prop :=
 | wfaenil: WFaEnv nil
 | wfaecons: forall ec, WFaEc ec -> forall p, WFaEnv p -> 
@@ -84,9 +83,7 @@ Qed.
 
 (*** Common functions for evaluation ***)
 
-(** Lookup an entry in the environment
-*** axioms are currently not allowed
-**)
+(** Lookup an entry in the environment **)
 Inductive Lookup: string -> environ -> envClass -> Prop :=
 | LHit: forall s p t, Lookup s ((s,t)::p) t
 | LMiss: forall s1 s2 p t ec,
@@ -316,6 +313,7 @@ Inductive Crct: environ -> nat -> Term -> Prop :=
 | CrctFix: forall n p ds m,
              Crct p n prop ->    (** convenient for IH *)
              CrctDs p (n + dlength ds) ds -> Crct p n (TFix ds m)
+| CrctAx: forall n p ty, Crct p n ty -> Crct p n (TAx ty)
 | CrctInd: forall n p ind, Crct p n prop -> Crct p n (TInd ind)
 with Crcts: environ -> nat -> Terms -> Prop :=
 | CrctsNil: forall n p, Crct p n prop -> Crcts p n tnil
@@ -348,7 +346,7 @@ Lemma Crct_WFTrm:
   (forall p n ts, Crcts p n ts -> WFTrms ts n) /\
   (forall (p:environ) (n:nat) (ds:Defs), CrctDs p n ds -> WFTrmDs ds n) /\
   (forall (p:environ) (n:nat) (itp:itypPack), CrctTyp p n itp -> True).
-apply CrctCrctsCrctDsTyp_ind; intros; try auto; try (solve [constructor]).
+apply CrctCrctsCrctDsTyp_ind; intros; auto.
 Qed.
 
 Lemma Crct_mkApp_ident:
@@ -382,6 +380,7 @@ apply CrctCrctsCrctDsTyp_ind; intros.
 - eapply CrctConstruct; eassumption.
 - apply CrctCase; assumption.
 - apply CrctFix; assumption.
+- apply CrctAx; assumption.
 - apply CrctInd; assumption.
 - apply CrctsNil; assumption.
 - apply CrctsCons; assumption.
@@ -682,6 +681,8 @@ eapply CrctCrctsCrctDsTyp_ind; intros; auto.
 - apply CrctFix.
   + eapply H0. eassumption. intros h. inversion h.
   + eapply H2. eassumption. intros h. elim H4. apply PoFix. assumption.
+- apply CrctAx. apply (H0 _ _ _ H1). intros h. elim H2.
+  apply PoAx. assumption.
 - apply CrctInd. apply (H0 _ _ _ H1). inversion 1. 
 - apply CrctsNil. rewrite H1 in H. inversion H; assumption.
 - apply CrctsCons.
@@ -871,6 +872,15 @@ induction 1; intros; try discriminate.
 - injection H1; intros; subst. assumption.
 Qed.
 
+Lemma Crct_invrt_Ax:
+  forall p n t, Crct p n t ->
+  forall u, t = (TAx u) -> Crct p n u.
+induction 1; intros; try discriminate.
+- apply (proj1 Crct_weaken); intuition.
+- specialize (IHCrct _ H2). apply (proj1 Crct_Typ_weaken); intuition.
+- myInjection H0. assumption.
+Qed.
+  
 Lemma Crct_invrt_Construct:
   forall p n construct, Crct p n construct ->
   forall ipkgNm inum cnum, construct = (TConstruct (mkInd ipkgNm inum) cnum) ->
@@ -964,7 +974,7 @@ Proof.
     + destruct H3 as [x [h1 h2]]. eapply (@CrctConst _ _ x); trivial.
       * eapply Crct_Sort. eassumption.
   - apply CrctInd. eapply Crct_Sort. eassumption.
-  - destruct ind.  edestruct (Crct_invrt_Construct H0).
+  - destruct ind. edestruct (Crct_invrt_Construct H0).
     + reflexivity.
     + destruct H3 as [x [h1 h2]]. eapply CrctConstruct; try eassumption.
       * eapply Crct_Sort. eassumption.
@@ -979,6 +989,8 @@ Proof.
       * simpl in j. generalize (dlength d). induction n0.
         rewrite <- plus_n_O. assumption.
         rewrite <- plus_n_Sm. apply (proj1 Crct_up). assumption.
+  - apply CrctAx. apply H; try assumption.
+    apply (Crct_invrt_Ax H1 eq_refl).
   - apply CrctsNil. eapply Crct_Sort. eassumption.
   - inversion_Clear H2. apply CrctsCons.
     + apply H; trivial.
